{
  "@context": {
    "spdci": "https://schema.spdci.org/common/v1/",
    "rdfs": "http://www.w3.org/2000/01/rdf-schema#",
    "xsd": "http://www.w3.org/2001/XMLSchema#"
  },
  "@id": "spdci:Authorize",
  "@type": "rdfs:Class",
  "rdfs:comment": "The Authorize object that captures information about the authorization granted for data access or processing.",
  "rdfs:property": [
    {
      "@id": "spdci:ts",
      "@type": "rdfs:Datatype",
      "rdfs:domain": "spdci:Authorize",
      "rdfs:range": "xsd:dateTime",
      "rdfs:comment": "Timestamp indicating when the authorization was granted."
    },
    {
      "@id": "spdci:purpose",
      "@type": "rdfs:Class",
      "rdfs:domain": "spdci:Authorize",
      "rdfs:comment": "Object describing the purpose for which authorization is granted.",
      "rdfs:property": [
        {
          "@id": "spdci:code",
          "@type": "rdfs:Datatype",
          "rdfs:domain": "spdci:purpose",
          "rdfs:range": "xsd:string",
          "rdfs:comment": "Code representing the authorization purpose, from a fixed set defined at the reference URI."
        },
        {
          "@id": "spdci:text",
          "@type": "rdfs:Datatype",
          "rdfs:domain": "spdci:purpose",
          "rdfs:range": "xsd:string",
          "rdfs:comment": "Human-readable description of the authorization purpose."
        },
        {
          "@id": "spdci:ref_uri",
          "@type": "rdfs:Datatype",
          "rdfs:domain": "spdci:purpose",
          "rdfs:range": "xsd:anyURI",
          "rdfs:comment": "URI providing more information about the authorization codes."
        }
      ]
    }
  ]
}
