{
  "@context": {
    "spdci": "https://schema.spdci.org/common/v1/",
    "rdfs": "http://www.w3.org/2000/01/rdf-schema#",
    "xsd": "http://www.w3.org/2001/XMLSchema#"
  },
  "@id": "spdci:MsgCallbackHeader",
  "@type": "rdfs:Class",
  "rdfs:comment": "Message header",
  "rdfs:label": "Message Header",
  "rdfs:subClassOf": [
    {
      "@type": "rdfs:Class",
      "rdfs:label": "Structured Entity"
    }
  ],
  "rdfs:property": [
    {
      "@id": "spdci:version",
      "@type": "rdfs:Datatype",
      "rdfs:domain": "spdci:MsgCallbackHeader",
      "rdfs:range": "xsd:string",
      "rdfs:comment": "Messaging protocol specification version being used"
    },
    {
      "@id": "spdci:message_id",
      "@type": "rdfs:Datatype",
      "rdfs:domain": "spdci:MsgCallbackHeader",
      "rdfs:range": "xsd:string",
      "rdfs:comment": "Unique message id to communicate between sender and receiver systems to reliable deliver the message over any transport layer i.e https, pub/sub, sftp etc."
    },
    {
      "@id": "spdci:message_ts",
      "@type": "rdfs:Datatype",
      "rdfs:domain": "spdci:MsgCallbackHeader",
      "rdfs:range": "spdci:DateTime"
    },
    {
      "@id": "spdci:action",
      "@type": "rdfs:Datatype",
      "rdfs:domain": "spdci:MsgCallbackHeader",
      "rdfs:range": "xsd:string",
      "rdfs:comment": "G2P Connect specific action. Usually verb from the URI. Helps in sync, async, store/fwd processing."
    },
    {
      "@id": "spdci:status",
      "@type": "rdfs:Datatype",
      "rdfs:domain": "spdci:MsgCallbackHeader",
      "rdfs:range": {
        "@id": "spdci:RequestStatus"
      }
    },
    {
      "@id": "spdci:status_reason_code",
      "@type": "rdfs:Datatype",
      "rdfs:domain": "spdci:MsgCallbackHeader",
      "rdfs:range": {
        "@id": "spdci:MsgHeaderStatusReasonCodeEnum"
      }
    },
    {
      "@id": "spdci:status_reason_message",
      "@type": "rdfs:Datatype",
      "rdfs:domain": "spdci:MsgCallbackHeader",
      "rdfs:range": "xsd:string",
      "rdfs:comment": "Status reason code message, if any, Helps actionable messaging for system/end users."
    },
    {
      "@id": "spdci:total_count",
      "@type": "rdfs:Datatype",
      "rdfs:domain": "spdci:MsgCallbackHeader",
      "rdfs:range": "xsd:integer",
      "rdfs:comment": "Total no of requests present in the message request."
    },
    {
      "@id": "spdci:completed_count",
      "@type": "rdfs:Datatype",
      "rdfs:domain": "spdci:MsgCallbackHeader",
      "rdfs:range": "xsd:integer",
      "rdfs:comment": "No of requests in completed state. Complete includes success and error requests due to functional errors."
    },
    {
      "@id": "spdci:sender_id",
      "@type": "rdfs:Datatype",
      "rdfs:domain": "spdci:MsgCallbackHeader",
      "rdfs:range": "xsd:string",
      "rdfs:comment": "sender_id registered with the receiving system or gateway."
    },
    {
      "@id": "spdci:receiver_id",
      "@type": "rdfs:Datatype",
      "rdfs:domain": "spdci:MsgCallbackHeader",
      "rdfs:range": "xsd:string",
      "rdfs:comment": "Receiver id registered with the calling system. Used for authorization, encryption, digital sign verification, etc., functions"
    },
    {
      "@id": "spdci:is_msg_encrypted",
      "@type": "rdfs:Datatype",
      "rdfs:domain": "spdci:MsgCallbackHeader",
      "rdfs:range": "xsd:boolean",
      "rdfs:comment": "Is message encrypted?"
    },
    {
      "@id": "spdci:meta",
      "@type": "rdfs:Datatype",
      "rdfs:domain": "spdci:MsgCallbackHeader",
      "rdfs:range": "spdci:Meta"
    }
  ]
}

