{
  "@context": {
    "spdci": "https://schema.spdci.org/common/v1/",
    "rdfs": "http://www.w3.org/2000/01/rdf-schema#",
    "xsd": "http://www.w3.org/2001/XMLSchema#"
  },
  "@id": "spdci:Address",
  "@type": "rdfs:Class",
  "rdfs:comment": "An address is a structured entity that represents the details and components of an address.",
  "rdfs:subClassOf": [
    {
      "@type": "rdfs:Class",
      "rdfs:label": "Structured Entity"
    }
  ],
  "rdfs:property": [
    {
      "@id": "spdci:address_line_1",
      "@type": "rdfs:Datatype",
      "rdfs:domain": "spdci:Address",
      "rdfs:range": "xsd:string",
      "rdfs:comment": "Full mailing address, formatted for display or use on a mailing label."
    },
    {
      "@id": "spdci:address_line_2",
      "@type": "rdfs:Datatype",
      "rdfs:domain": "spdci:Address",
      "rdfs:range": "xsd:string",
      "rdfs:comment": "Full street address component, which may include house number, street name, Post Office Box, and multi-line extended street address information."
    },
    {
      "@id": "spdci:locality",
      "@type": "rdfs:Datatype",
      "rdfs:domain": "spdci:Address",
      "rdfs:range": "xsd:string",
      "rdfs:comment": "City or locality component."
    },
    {
      "@id": "spdci:sub_region_code",
      "@type": "rdfs:Datatype",
      "rdfs:domain": "spdci:Address",
      "rdfs:range": "xsd:string",
      "rdfs:comment": "District or sub-regional code."
    },
    {
      "@id": "spdci:region_code",
      "@type": "rdfs:Datatype",
      "rdfs:domain": "spdci:Address",
      "rdfs:range": "xsd:string",
      "rdfs:comment": "State, province, prefecture, or region component."
    },
    {
      "@id": "spdci:postal_code",
      "@type": "rdfs:Datatype",
      "rdfs:domain": "spdci:Address",
      "rdfs:range": "xsd:string",
      "rdfs:comment": "Zip Code or postal code component."
    },
    {
      "@id": "spdci:country_code",
      "@type": "rdfs:Datatype",
      "rdfs:domain": "spdci:Address",
      "rdfs:range": "xsd:string",
      "rdfs:comment": "Country part of an address."
    },
    {
      "@id": "spdci:geo_location",
      "@type": "rdfs:Datatype",
      "rdfs:domain": "spdci:Address",
      "rdfs:range": "spdci:GeoLocation"
    }
  ]
}
