{
  "@context": {
    "@vocab": "http://spdci.org/schemas/common/v1",
    "xsd": "http://www.w3.org/2001/XMLSchema#",
    "schema": "http://schema.org/",
    "rdfs": "http://www.w3.org/2000/01/rdf-schema#",
    "owl": "http://www.w3.org/2002/07/owl#"
  },
  "@graph": [
    {
      "rdfs:subClassOf": "rdfs:Resource",
      "@id": "spdci:CRVS_Person",
      "@type": "rdfs:Class",
      "rdfs:comment": "Represents a person in a Civil Registration and Vital Statistics context.",
      "rdfs:property": [
        {
          "@id": "spdci:identifier",
          "@type": "rdfs:Datatype",
          "rdfs:domain": "spdci:CRVS_Person",
          "rdfs:range": "@id",
          "rdfs:comment": "Applicant's identifier in the CRVS system using URI format."
        },
        {
          "@id": "spdci:name",
          "@type": "rdfs:ObjectProperty",
          "rdfs:domain": "spdci:CRVS_Person",
          "rdfs:range": "spdci:Name",
          "rdfs:comment": "Full name in a displayable form, including possible titles and suffixes. Formatted according to the applicant's locale norms and/or preferences."
        },
        {
          "@id": "spdci:phone_number",
          "@type": "rdfs:Datatype",
          "rdfs:domain": "spdci:CRVS_Person",
          "rdfs:range": "xsd:string",
          "rdfs:comment": "Applicant's preferred phone number. The format E.164 is recommended."
        },
        {
          "@id": "spdci:email",
          "@type": "rdfs:Datatype",
          "rdfs:domain": "spdci:CRVS_Person",
          "rdfs:range": "xsd:string",
          "rdfs:comment": "Applicant's preferred email address. The format must comply with RFC 5322 addr-spec."
        },
        {
          "@id": "spdci:sex",
          "rdfs:comment": "Sex of the applicant, represented as an enumeration (Male, Female, Others, Unknown).",
          "@type": "rdfs:Datatype",
          "rdfs:domain": "spdci:CRVS_Person",
          "rdfs:range": "spdci:SexEnum"
        },
        {
          "@id": "spdci:birthdate",
          "rdfs:comment": "The date of birth of the applicant, formatted according to schema:DateTime.",
          "@type": "rdfs:Datatype",
          "rdfs:domain": "spdci:CRVS_Person",
          "rdfs:range": "schema:DateTime"
        },
        {
          "@id": "spdci:birthplace",
          "rdfs:comment": "Physical location where the applicant was born, represented as an address object.",
          "@type": "rdfs:ObjectProperty",
          "rdfs:domain": "spdci:CRVS_Person",
          "rdfs:range": "spdci:Place"
        },
        {
          "@id": "spdci:deathdate",
          "rdfs:comment": "The date of death of the applicant, if applicable. Formatted according to schema:DateTime.",
          "@type": "rdfs:Datatype",
          "rdfs:domain": "spdci:CRVS_Person",
          "rdfs:range": "schema:DateTime"
        },
        {
          "@id": "spdci:deathplace",
          "rdfs:comment": "Physical location where the applicant died, if applicable. Represented as an address object.",
          "@type": "rdfs:ObjectProperty",
          "rdfs:domain": "spdci:CRVS_Person",
          "rdfs:range": "spdci:Place"
        },
        {
          "@id": "spdci:address",
          "rdfs:comment": "Current residential address of the applicant, represented as an address object.",
          "@type": "rdfs:ObjectProperty",
          "rdfs:domain": "spdci:CRVS_Person",
          "rdfs:range": "spdci:Place"
        },
        {
          "@id": "spdci:marital_status",
          "rdfs:comment": "Current marital status of the applicant, represented as an enumeration (e.g., Married, Divorced, etc.).",
          "@type": "rdfs:ObjectProperty",
          "rdfs:domain": "spdci:CRVS_Person",
          "rdfs:range": "spdci:MaritalStatusEnum"
        },
        {
          "@id": "spdci:marriagedate",
          "rdfs:comment": "Date when the applicant got married, if applicable. Formatted according to schema:DateTime.",
          "@type": "rdfs:Datatype",
          "rdfs:domain": "spdci:CRVS_Person",
          "rdfs:range": "schema:DateTime"
        },
        {
          "@id": "spdci:divorcedate",
          "rdfs:comment": "Date when the applicant got divorced, if applicable. Formatted according to schema:DateTime.",
          "@type": "rdfs:Datatype",
          "rdfs:domain": "spdci:CRVS_Person",
          "rdfs:range": "schema:DateTime"
        },
        {
          "@id": "spdci:relations",
          "@type": "rdfs:ObjectProperty",
          "rdfs:domain": "spdci:CRVS_Person",
          "rdfs:range": "spdci:Relationship",
          "rdfs:comment": "Relationships the applicant has with other persons, represented as an array of relationship objects."
        }
      ]
    },
    {
      "@id": "spdci:MaritalStatusEnum",
      "@type": "rdfs:Class",
      "rdfs:comment": "Enumeration for marital status.",
      "rdfs:subClassOf": "rdfs:Resource",
      "owl:oneOf": [
        "spdci:NeverMarried",
        "spdci:Married",
        "spdci:Widow",
        "spdci:Annulled",
        "spdci:Divorced",
        "spdci:LegallySeparated",
        "spdci:Unmarried"
      ]
    },
    {
      "@id": "spdci:marital_status",
      "@type": "rdf:Property",
      "rdfs:comment": "The marital status of a person.",
      "rdfs:domain": "spdci:CRVS_Person",
      "rdfs:range": "spdci:MaritalStatusEnum"
    },
    {
      "@id": "spdci:NeverMarried",
      "@type": "spdci:MaritalStatusEnum",
      "rdfs:label": "Never Married",
      "rdfs:comment": "No marriage contract has ever been entered"
    },
    {
      "@id": "spdci:Married",
      "@type": "spdci:MaritalStatusEnum",
      "rdfs:label": "Married",
      "rdfs:comment": "A current marriage contract is active"
    },
    {
      "@id": "spdci:Widow",
      "@type": "spdci:MaritalStatusEnum",
      "rdfs:label": "Widow",
      "rdfs:comment": "The spouse has died"
    },
    {
      "@id": "spdci:Annulled",
      "@type": "spdci:MaritalStatusEnum",
      "rdfs:label": "Annulled",
      "rdfs:comment": "Marriage contract has been declared null and to not have existed"
    },
    {
      "@id": "spdci:Divorced",
      "@type": "spdci:MaritalStatusEnum",
      "rdfs:label": "Divorced",
      "rdfs:comment": "Marriage contract has been declared dissolved and inactive"
    },
    {
      "@id": "spdci:LegallySeparated",
      "@type": "spdci:MaritalStatusEnum",
      "rdfs:label": "Legally Separated",
      "rdfs:comment": "Legally Separated"
    },
    {
      "@id": "spdci:Unmarried",
      "@type": "spdci:MaritalStatusEnum",
      "rdfs:label": "Unmarried",
      "rdfs:comment": "The person is not presently married. The marital history is not known or stated."
    },
    {
      "@id": "spdci:SexEnum",
      "@type": "rdfs:Class",
      "rdfs:comment": "Enumeration for sex.",
      "rdfs:subClassOf": "rdfs:Resource",
      "owl:oneOf": [
        "spdci:Male",
        "spdci:Female",
        "spdci:Others",
        "spdci:Unknown"
      ]
    },
    {
      "@id": "spdci:Male",
      "@type": "spdci:SexEnum",
      "rdfs:label": "male",
      "rdfs:comment": "Male"
    },
    {
      "@id": "spdci:Female",
      "@type": "spdci:SexEnum",
      "rdfs:label": "female",
      "rdfs:comment": "Female"
    },
    {
      "@id": "spdci:Others",
      "@type": "spdci:SexEnum",
      "rdfs:label": "other",
      "rdfs:comment": "Others"
    },
    {
      "@id": "spdci:Unknown",
      "@type": "spdci:SexEnum",
      "rdfs:label": "unknown",
      "rdfs:comment": "Unknown"
    }
  ]
}
