{
  "@context": {
    "spdci": "http://spdci.org/schemas/common/v1/",
    "rdfs": "http://www.w3.org/2000/01/rdf-schema#",
    "schema": "http://schema.org/",
    "xsd": "http://www.w3.org/2001/XMLSchema#"
  },
  "@graph": [
    {
      "@id": "spdci:GeoCoordinates",
      "@type": "rdfs:Class",
      "rdfs:comment": "A geographical coordinate set defined by a latitude and a longitude according to the WGS 84 system.",
      "rdfs:property": [
        {
          "@id": "spdci:latitude",
          "@type": "rdf:Property",
          "rdfs:comment": "The latitude of a location. For example ```37.42242``` ([WGS 84](https://en.wikipedia.org/wiki/World_Geodetic_System)).",
          "rdfs:label": "latitude",
          "rdfs:domain": "spdci:GeoCoordinates",
          "rdfs:range": "xsd:decimal"
        },
        {
          "@id": "spdci:longitude",
          "@type": "rdf:Property",
          "rdfs:comment": "The longitude of a location. For example ```-122.08585``` ([WGS 84](https://en.wikipedia.org/wiki/World_Geodetic_System)).",
          "rdfs:label": "longitude",
          "rdfs:domain": "spdci:GeoCoordinates",
          "rdfs:range": "xsd:decimal"
        }
      ]
    }
  ]
}
