{
  "@context": {
    "spdci": "https://schema.spdci.org/common/v1/",
    "rdfs": "http://www.w3.org/2000/01/rdf-schema#",
    "xsd": "http://www.w3.org/2001/XMLSchema#"
  },
  "@id": "spdci:GeoShape",
  "@type": "rdfs:Class",
  "rdfs:comment": "GeoShape represents a geometrical shape on a map, defined by various properties like box, circle, elevation, line, and polygon.",
  "rdfs:subClassOf": [
    {
      "@type": "rdfs:Class",
      "rdfs:label": "Structured Entity"
    }
  ],
  "rdfs:property": [
    {
      "@id": "spdci:box",
      "@type": "rdfs:Datatype",
      "rdfs:domain": "spdci:GeoShape",
      "rdfs:range": "xsd:string",
      "rdfs:comment": "Defines a rectangular area on a map via two geographical points: the lower and upper corners."
    },
    {
      "@id": "spdci:circle",
      "@type": "rdfs:Datatype",
      "rdfs:domain": "spdci:GeoShape",
      "rdfs:range": "xsd:string",
      "rdfs:comment": "Specifies a circular region with a defined radius, centered at a given latitude and longitude. Expressed as a pair followed by a radius in meters."
    },
    {
      "@id": "spdci:elevation",
      "@type": "rdfs:Datatype",
      "rdfs:domain": "spdci:GeoShape",
      "rdfs:range": "xsd:string",
      "rdfs:comment": "Indicates the elevation of a location (WGS 84)."
    },
    {
      "@id": "spdci:line",
      "@type": "rdfs:Datatype",
      "rdfs:domain": "spdci:GeoShape",
      "rdfs:range": "xsd:string",
      "rdfs:comment": "Represents a point-to-point path defined by two or more points, expressed as a series of point objects separated by space."
    },
    {
      "@id": "spdci:polygon",
      "@type": "rdfs:Datatype",
      "rdfs:domain": "spdci:GeoShape",
      "rdfs:range": "xsd:string",
      "rdfs:comment": "Encloses an area with a point-to-point path, where the starting and ending points are identical. Expressed as a series of four or more space-delimited points, with the first and final points being identical."
    }
  ]
}
