{
  "@context": {
    "spdci": "http://spdci.org/schemas/common/v1/",
    "rdfs": "http://www.w3.org/2000/01/rdf-schema#",
    "xsd": "http://www.w3.org/2001/XMLSchema#"
  },
  "@id": "spdci:Place",
  "@type": "rdfs:Class",
  "rdfs:comment": "A place is a structured entity that represents the details and components of a location.",
  "rdfs:subClassOf": [
    {
      "@type": "rdfs:Class",
      "rdfs:label": "Structured Entity"
    }
  ],
  "rdfs:property": [
    {
      "@id": "spdci:identifier",
      "@type": "rdfs:Datatype",
      "rdfs:domain": "spdci:Place",
      "rdfs:range": "@id",
      "rdfs:comment": "Place identifier in another system such as the HDX location identifier https://data.humdata.org/."
    },
    {
      "@id": "spdci:name",
      "@type": "rdfs:Datatype",
      "rdfs:domain": "spdci:Place",
      "rdfs:range": "xsd:string",
      "rdfs:comment": "Full mailing address, formatted for display or use on a mailing label. This field may contain multiple lines, separated by newlines."
    },
    {
      "@id": "spdci:address",
      "@type": "rdfs:Datatype",
      "rdfs:domain": "spdci:Place",
      "rdfs:range": "xsd:string",
      "rdfs:comment": "Full mailing address, formatted for display or use on a mailing label. This field may contain multiple lines, separated by newlines."
    },
    {
      "@id": "spdci:geo",
      "@type": "rdfs:Datatype",
      "rdfs:domain": "spdci:Place",
      "rdfs:range": [
        "spdci:GeoCoordinates",
        "spdci:GeoShape"
      ],
      "rdfs:comment": "Geo Location details."
    },
    {
      "@id": "spdci:containedInPlace",
      "@type": "rdfs:Datatype",
      "rdfs:domain": "spdci:Place",
      "rdfs:range": "spdci:Place",
      "rdfs:comment": "A relationship indicating a larger place that this place is part of."
    },
    {
      "@id": "spdci:containsPlace",
      "@type": "rdfs:Datatype",
      "rdfs:domain": "spdci:Place",
      "rdfs:range": "spdci:Place",
      "rdfs:comment": "A relationship indicating a smaller place that is contained within this place."
    }
  ]
}
