{
  "@context": {
    "spdci": "http://spdci.org/schemas/src/extensions/openid/v1/",
    "rdfs": "http://www.w3.org/2000/01/rdf-schema#",
    "xsd": "http://www.w3.org/2001/XMLSchema#",
    "owl": "http://www.w3.org/2002/07/owl#"
  },
  "@id": "spdci:Issuer",
  "@type": "rdfs:Class",
  "rdfs:comment": "JSON object containing information about the issuer of this document.",
  "rdfs:label": "Issuer",
  "rdfs:subClassOf": [
    {
      "@type": "rdfs:Class",
      "rdfs:label": "Structured Entity"
    }
  ],
  "rdfs:property": [
    {
      "@id": "spdci:name",
      "@type": "rdfs:Datatype",
      "rdfs:domain": "spdci:Issuer",
      "rdfs:range": "xsd:string",
      "rdfs:comment": "Designation of the issuer of the document."
    },
    {
      "@id": "spdci:address",
      "@type": "rdfs:Datatype",
      "rdfs:domain": "spdci:Issuer",
      "rdfs:range": "spdci:Address",
    },
    {
      "@id": "spdci:country_code",
      "@type": "rdfs:Datatype",
      "rdfs:domain": "spdci:Issuer",
      "rdfs:range": "xsd:string",
      "rdfs:comment": "String denoting the country or supranational organization that issued the document as ISO 3166/ICAO 3-letter codes [ICAO-Doc9303].",
      "rdfs:examples" :" USA or JPN ."
    },
    {
      "@id": "spdci:jurisdiction",
      "@type": "rdfs:Datatype",
      "rdfs:domain": "spdci:Issuer",
      "rdfs:range": "xsd:string",
      "rdfs:comment": "String containing the name of the region(s)/state(s)/province(s)/municipality(ies) that issuer has jurisdiction over (if this information is not common knowledge or derivable from the address)."
    }
  ]
}