{
    "@context": {
        "spdci": "https://schema.spdci.org/extensions/fr/v1/data",
        "code": "https://schema.spdci.org/extensions/fr/v1/code",
        "xsd": "http://www.w3.org/2001/XMLSchema#",
        "spdcicore": "https://schema.spdci.org/core/v1/data",
        "spdcicode": "https://schema.spdci.org/core/v1/code",
        "rdfs": "http://www.w3.org/2000/01/rdf-schema#",
        "owl": "http://www.w3.org/2002/07/owl#"
    },
    "@id": "spdci:Farming_Activities",
    "@type": "rdfs:Class",
    "rdfs:comment": "This data object contains the information on people  held in the farmer registry",
    "rdfs:label": "Farming_Activities",
    "rdfs:subClassOf": [
      {
        "@type": "rdfs:Class",
        "rdfs:label": "Structured Entity"
      }
    ],
    "rdfs:property": [
        {
            "@id": "spdci:crop_production",
            "@type": "rdfs:Datatype",
            "rdfs:domain": "spdci:Farming_Activities",
            "rdfs:range": {
                "@id": "spdci:CropDetails",
                "@type": "rdfs:Class",
                "@container": "@list"
            },
            "rdfs:comment": "Group 011 -13: Crop production activities"
        },
        {
          "@id": "spdci:animal_production",
          "@type": "rdfs:Datatype",
          "rdfs:domain": "spdci:Farming_Activities",
          "rdfs:range": {
              "@id": "spdci:livestockDetails",
              "@type": "rdfs:Class",
              "@container": "@list"
          },
          "rdfs:comment": "Group 014: Animal productions"
        },
        {
          "@id": "spdci:mixed_farming",
          "@type": "rdfs:Datatype",
          "rdfs:domain": "spdci:CropDetails",
          "rdfs:range": "xsd:boolean",
          "rdfs:comment": "Group 015: Mixed farming, Includes both crops and animal related farming activities Yes (1) or No (0)."
        },
        {
            "@id": "spdci:agri_support_activities",
            "@type": "rdfs:Datatype",
            "rdfs:domain": "spdci:Farming_Activities",
            "rdfs:range": {
                "@id": "code:AgriSupportActivityEnum",
                "@type": "rdfs:Class",
                "@container": "@list"
            },
            "rdfs:comment": "Group 016: Support activities to agriculture and post-harvest crop activities"
        },
        {
            "@id": "spdci:aquaculture",
            "@type": "rdfs:Datatype",
            "rdfs:domain": "spdci:Farming_Activities",
            "rdfs:range": {
                "@id": "code:AquaCultureEnum",
                "@type": "rdfs:Class",
                "@container": "@list"
            },
            "rdfs:comment": "Group 032: Aquaculture"
        },
        {
            "@id": "spdci:aqua_support_activities",
            "@type": "rdfs:Datatype",
            "rdfs:domain": "spdci:Farming_Activities",
            "rdfs:range": "code:AquaSupportActivityEnum",
            "rdfs:comment": "Group 033: Support activities for fishing and aquaculture"
        },
        {
          "@id": "spdci:agroforestry",
          "@type": "rdfs:Datatype",
          "rdfs:domain": "spdci:Farming_Activities",
          "rdfs:range": {
              "@id": "code:ForestActivityEnum",
              "@type": "rdfs:Class",
              "@container": "@list"
          },
          "rdfs:comment": "The forest activity on the farm"
      },
        {
            "@id": "spdci:registration_date",
            "@type": "rdfs:Datatype",
            "rdfs:domain": "spdci:Farming_Activities",
            "rdfs:range": "spdcicore:DateTime",
            "rdfs:comment": "The date of registration of the applicant, formatted according to schema:DateTime."
          },
          {
            "@id": "spdci:last_updated",
            "@type": "rdfs:Datatype",
            "rdfs:domain": "spdci:Farming_Activities",
            "rdfs:range": "spdcicore:DateTime",
            "rdfs:comment": "The date when person details got updated , formatted according to schema:DateTime."
          }
      
    ]
  }
  