{
    "@context": {
      "spdci": "https://schema.spdci.org/extensions/social/v1/",
      "rdfs": "http://www.w3.org/2000/01/rdf-schema#",
      "xsd": "http://www.w3.org/2001/XMLSchema#",
      "owl": "http://www.w3.org/2002/07/owl#",
      "common": "https://schema.spdci.org/common/v1/"
    },
    "@id": "spdci:DisabilityInfo",
    "@type": "rdfs:Class",
    "rdfs:comment": "This data object contains the information on people and households held in the social registry.",
    "rdfs:label": "DisabilityInfo",
    "rdfs:subClassOf": [
      {
        "@type": "rdfs:Class",
        "rdfs:label": "Structured Entity"
      }
    ],
    "rdfs:property": [
        {
            "@id": "spdci:disability_type",
            "@type": "rdfs:Datatype",
            "rdfs:domain": "spdci:DisabilityInfo",
            "rdfs:range": {
                "@id": "spdci:DisabilityTypeEnum",
                "@type": "xsd:string"
            },
            "rdfs:comment": "The specific type of disability the individual has. For example, H54.0 might represent a particular type of visual impairment."
          },
          {
            "@id": "spdci:functional_limitation_type",
            "@type": "rdfs:Datatype",
            "rdfs:domain": "spdci:DisabilityInfo",
            "rdfs:range":  {
              "@type": "xsd:string"
      
            },
            "rdfs:comment": "Describes the type of functional limitation experienced by the individual."
          },
          {
            "@id": "spdci:functional_severity",
            "@type": "rdfs:Datatype",
            "rdfs:domain": "spdci:DisabilityInfo",
            "rdfs:range": {
             "@type": "xsd:string"
            },
            "rdfs:comment": "Indicates the severity level of the functional limitation."
          }
    ],
    "required": ["@context","@type","spdci:disability_type"]
  }