{
    "@context": {
      "spdci": "https://schema.spdci.org/extensions/social/v1/",
      "rdfs": "http://www.w3.org/2000/01/rdf-schema#",
      "xsd": "http://www.w3.org/2001/XMLSchema#",
      "owl": "http://www.w3.org/2002/07/owl#",
      "schema": "http://schema.org/"
    },
    "@id": "spdci:Group",
    "@type": "rdfs:Class",
    "rdfs:comment": "A group unit represents a group of related individuals in the social registry",
    "rdfs:label": "Group",
    "rdfs:subClassOf": [
      {
        "@type": "rdfs:Class",
        "rdfs:label": "Structured Entity"
      }
    ],
    "rdfs:property": [
      {
        "@id": "spdci:group_identifier",
        "@type": "rdfs:Datatype",
        "rdfs:domain": "spdci:Group",
        "rdfs:range": {
          "@id": "spdci:Identifier",
          "@type": "rdfs:Class",
          "@container": "@list"
        },
        "rdfs:comment": "A unique identifier assigned to each individual."
      },
      {
        "@id": "spdci:group_type",
        "@type": "rdfs:Datatype",
        "rdfs:domain": "spdci:Group",
        "rdfs:range": "common:GroupTypeEnum",
        "rdfs:comment": "The entity representing the group"
      },
      {
        "@id": "spdci:geographical_location",
        "rdfs:comment": "Physical location where the group is living",
        "@type": "rdfs:Datatype",
        "rdfs:domain": "spdci:Group",
        "rdfs:range": "common:Place"
      },
      {
        "@id": "spdci:address",
        "@type": "rdfs:Datatype",
        "rdfs:domain": "spdci:Group",
        "rdfs:range": {
             "@id": "spdci:Address",
             "@type": "rdfs:Class",
             "@container":"@list"
        },
        "rdfs:comment": "Current residential address of the group, represented as an address object."
      },
      {
        "@id": "spdci:place_address",
        "@type": "rdfs:Datatype",
        "rdfs:domain": "spdci:Member",
        "rdfs:range": "xsd:boolean",
        "rdfs:comment": "added place or address? place (1) or address (0)."
      },
      {
        "@id": "spdci:poverty_score",
        "@type": "rdfs:Datatype",
        "rdfs:domain": "spdci:Group",
        "rdfs:range": "xsd:decimal",
        "rdfs:comment": "A metric generated based on the assessment of various group characteristics."
      },
      {
        "@id": "spdci:poverty_score_type",
        "@type": "rdfs:Datatype",
        "rdfs:domain": "spdci:Group",
        "rdfs:range": "xsd:string",  
        "rdfs:comment": "The types of poverty scores that are is to measure and categorize the level of poverty."
      },
      {
        "@id": "spdci:group_head_info",
        "@type": "rdfs:Datatype",
        "rdfs:domain": "spdci:Group",
        "rdfs:range": {
             "@id": "spdci:Member",
             "@type": "rdfs:Class"
        },
        "rdfs:comment": "Personal details of the head of the group."
      },
      {
        "@id": "spdci:group_size",
        "@type": "rdfs:Datatype",
        "rdfs:domain": "spdci:Group",
        "rdfs:range": "xsd:integer",
        "rdfs:comment": "The total number of members in the group."
      },
      {
        "@id": "spdci:member_list",
        "@type": "rdfs:Datatype",
        "rdfs:domain": "spdci:Group",
        "rdfs:range": {
          "@id": "spdci:Member",
          "@type": "rdfs:Class",
          "@container": "@list"
        },
        "rdfs:comment": "A list of the related individuals in a group."
      },
      {
        "@id": "spdci:registration_date",
        "@type": "rdfs:Datatype",
        "rdfs:domain": "spdci:Group",
        "rdfs:range": "common:DateTime",
        "rdfs:comment": "The date the details of the group were registered."
      },
      {
        "@id": "spdci:last_updated",
        "@type": "rdfs:Datatype",
        "rdfs:domain": "spdci:Group",
        "rdfs:range": "common:DateTime",
        "rdfs:comment": "The date the details of the group were last updated."
      },
      {
        "@id": "spdci:additional_attributes",
        "@type": "rdf:Property",
        "rdfs:domain": "spdci:Group",
        "rdfs:range": {
          "@type": "@id",
          "@container": "@list"
        },
        "rdfs:comment": "Additional attributes of the group, represented as a list of key-value pairs.",
        "schema:value": {
          "@type": "xsd:string"
        }
      }
    ] }
  