{
  "@context": {
    "spdci": "https://schema.spdci.org/extensions/social/v1/",
    "rdfs": "http://www.w3.org/2000/01/rdf-schema#",
    "xsd": "http://www.w3.org/2001/XMLSchema#",
    "owl": "http://www.w3.org/2002/07/owl#",
    "common": "https://schema.spdci.org/common/v1/"

  },
  "@id": "spdci:Household",
  "@type": "rdfs:Class",
  "rdfs:comment": "A household or other grouping representing a group of individual beneficiaries in the social registry.",
  "rdfs:label": "Household",
  "rdfs:subClassOf": [
    {
      "@type": "rdfs:Class",
      "rdfs:label": "Structured Entity"
    }
  ],
  "rdfs:property": [
    {
      "@id": "spdci:household_identifier",
      "@type": "rdfs:Datatype",
      "rdfs:domain": "spdci:Household",
      "rdfs:range": "common:Identifier",
      "rdfs:comment": "The unique identifier for a household."
    },
    {
      "@id": "spdci:group_type",
      "@type": "rdfs:Datatype",
      "rdfs:domain": "spdci:Household",
      "rdfs:range": "xsd:string",
      "rdfs:comment": "The type of group."
    },
    {
      "@id": "spdci:identifier",
      "@type": "rdfs:Datatype",
      "rdfs:domain": "spdci:Household",
      "rdfs:range": "common:Identifier",
      "rdfs:comment": "Identifier for one parent of the applicant. Must be a unique identifier similar to the applicant's identifier."
    },
    {
      "@id": "spdci:is_head",
      "@type": "rdfs:Datatype",
      "rdfs:domain": "spdci:Household",
      "rdfs:range": {
        "@id": "spdci:HeadEnum"
      },
      "rdfs:comment": "A designation for which member is the head of household."
    },
    {
      "@id": "spdci:is_disabled",
      "@type": "rdfs:Datatype",
      "rdfs:domain": "spdci:Household",
      "rdfs:range": "xsd:boolean",
      "rdfs:comment": "Specifies if the applicant is disabled, not disabled or not known."
    },
    {
      "@id": "spdci:household_size",
      "@type": "rdfs:Datatype",
      "rdfs:domain": "spdci:Household",
      "rdfs:range": "xsd:integer",
      "rdfs:comment": "The total number of members in the household."
    }
  ]
}
