{
  "@context": {
    "spdci": "https://schema.spdci.org/common/v1/",
    "rdfs": "http://www.w3.org/2000/01/rdf-schema#",
    "xsd": "http://www.w3.org/2001/XMLSchema#",
    "owl": "http://www.w3.org/2002/07/owl#",
    "schema": "http://schema.org/"
  },
  "@id": "spdci:Household",
  "@type": "rdfs:Class",
  "rdfs:comment": "A household or other grouping representing a group of individual beneficiaries in the social registry.",
  "rdfs:label": "Household",
  "rdfs:subClassOf": [
    {
      "@type": "rdfs:Class",
      "rdfs:label": "Structured Entity"
    }
  ],
  "rdfs:property": [
    {
      "@id": "spdci:household_identifier",
      "@type": "rdfs:Datatype",
      "rdfs:domain": "spdci:Household",
      "rdfs:range": "xsd:string",
      "rdfs:comment": "The unique identifier for a household."
    },
    {
      "@id": "spdci:address",
      "@type": "rdfs:Datatype",
      "rdfs:domain": "spdci:Household",
      "rdfs:range": {
           "@id": "spdci:Address",
           "@type": "rdfs:Class"
      },
      "rdfs:comment": "Current residential address of the applicant, represented as an address object."
    },
    {
      "@id": "spdci:poverty_score",
      "@type": "rdfs:Datatype",
      "rdfs:domain": "spdci:Household",
      "rdfs:range": "xsd:decimal",
      "rdfs:comment": "The poverty score assigned to the household as a result of a proxy means test or other poverty ranking approach."
    },
    {
      "@id": "spdci:poverty_score_type",
      "@type": "rdfs:Datatype",
      "rdfs:domain": "spdci:Household",
      "rdfs:range": "xsd:string",
      "rdfs:comment": "The types of poverty scores that are is to measure and categorize the level of poverty."
    },
    {
      "@id": "spdci:household_head_info",
      "@type": "rdfs:Datatype",
      "rdfs:range": {
           "@id": "spdci:Member",
           "@type": "rdfs:Class"
      },
      "rdfs:comment": "Personal details of the head of the household"
    },
    {
      "@id": "spdci:unit_size",
      "@type": "rdfs:Datatype",
      "rdfs:domain": "spdci:Household",
      "rdfs:range": "xsd:integer",
      "rdfs:comment": "The size of the unit in terms of number of members."
    },
    {
      "@id": "spdci:member_list",
      "@type": "rdfs:Datatype",
      "rdfs:domain": "spdci:Household",
      "rdfs:range": {
        "@id": "spdci:Member",
        "@type": "rdfs:Class",
        "@container": "@list"
      },
      "rdfs:comment": "An array of members belonging to the household."
    },
    {
      "@id": "spdci:registration_date",
      "@type": "rdfs:Datatype",
      "rdfs:domain": "spdci:Household",
      "rdfs:range": "common:DateTime",
      "rdfs:comment": "The date on which the household was first registered in the social registry."
    },
    {
      "@id": "spdci:last_updated",
      "@type": "rdfs:Datatype",
      "rdfs:domain": "spdci:Household",
      "rdfs:range": "common:DateTime",
      "rdfs:comment": "Date on which applicant data was last updated."
    },
    {
      "@id": "spdci:additional_attributes",
      "@type": "rdfs:Datatype",
      "rdfs:domain": "spdci:Household",
      "rdfs:range": {
        "@type": "xsd:string",
        "@container": "@list"
      },
      "rdfs:comment": "Additional attributes as an array of strings."
    }
  ],
  "required": ["@context","@type","spdci:household_identifier", "spdci:address", "spdci:household_head_info", "spdci:unit_size","spdci:member_list","spdci:registration_date"]
}
