{
  "@context": {
    "spdci": "https://schema.spdci.org/extensions/social/v1/",
    "rdfs": "http://www.w3.org/2000/01/rdf-schema#",
    "xsd": "http://www.w3.org/2001/XMLSchema#",
    "owl": "http://www.w3.org/2002/07/owl#",
    "common": "https://schema.spdci.org/common/v1/"
  },
  "@id": "spdci:Person",
  "@type": "rdfs:Class",
  "rdfs:comment": "This data object contains the information on people and households held in the social registry.",
  "rdfs:label": "Person",
  "rdfs:subClassOf": [
    {
      "@type": "rdfs:Class",
      "rdfs:label": "Structured Entity"
    }
  ],
  "rdfs:property": [
    {
      "@id": "spdci:identifier",
      "@type": "rdfs:Datatype",
      "rdfs:domain": "spdci:Person",
      "rdfs:range": {
           "@id": "common:Identifier",
           "@type": "rdfs:Class",
           "@container": "@list",
           "minitems": 1
      },
      "rdfs:comment": "The person's identification number."
    },
    {
      "@id": "spdci:name",
      "@type": "rdfs:Datatype",
      "rdfs:domain": "spdci:Person",
      "rdfs:range": {
           "@id": "common:Name",
           "@type": "rdfs:Class",
           "@container": "@list",
           "minitems": 1
      },
      "rdfs:comment": "Full name in a displayable form, possibly including titles and suffixes, in the order of the applicant's locale norms and/or preferences."
    },
    {
      "@id": "spdci:birth_date",
      "@type": "rdfs:Datatype",
      "rdfs:domain": "spdci:Person",
      "rdfs:range": "common:DateTime",
      "rdfs:comment": "The date of birth of the applicant, formatted according to schema:DateTime."
    },
    {
      "@id": "spdci:sex",
      "@type": "rdfs:Datatype",
      "rdfs:domain": "spdci:Person",
      "rdfs:range": "common:SexCategoryEnum",
      "rdfs:comment": "Sex of the applicant, represented as an enumeration ."
    },
    {
      "@id": "spdci:marital_status",
      "@type": "rdfs:Datatype",
      "rdfs:domain": "spdci:Person",
      "rdfs:range": "common:MaritalStatusEnum",
      "rdfs:comment": "The person's marital status"
    },
    {
      "@id": "spdci:is_disabled",
      "@type": "rdfs:Datatype",
      "rdfs:domain": "spdci:Person",
      "rdfs:range": "spdci:IsDisabledEnum",
      "rdfs:comment": "Specifies if the applicant is disabled, not disabled or not known."
    },
    {
      "@id": "spdci:disability_identifier",
      "@type": "rdfs:Datatype",
      "rdfs:domain": "spdci:Person",
      "rdfs:range": "common:Identifier",
      "rdfs:comment": "Identifier for the disability registry."
    },
    {
      "@id": "spdci:disability_type",
      "@type": "rdfs:Datatype",
      "rdfs:domain": "spdci:Person",
      "rdfs:range": {
          "@id": "spdci:DisabilityTypeEnum",
          "@type": "xsd:string",
          "@container": "@list"
      },
      "rdfs:comment": "Identifier for the disability registry."
    },
    {
      "@id": "spdci:functional_limitation_type",
      "@type": "rdfs:Datatype",
      "rdfs:domain": "spdci:Person",
      "rdfs:range":  {
        "@type": "xsd:string",
        "@container":"@list"

      },
      "rdfs:comment": "Functional limitation of the person."
    },
    {
      "@id": "spdci:functional_severity",
      "@type": "rdfs:Datatype",
      "rdfs:domain": "spdci:Person",
      "rdfs:range": {
       "@type": "xsd:string",
       "@container":"@list"
      },
      "rdfs:comment": "Functional severity of the person."
    },
    {
      "@id": "spdci:nationality",
      "@type": "rdfs:Datatype",
      "rdfs:domain": "spdci:Person",
      "rdfs:range": {
       "@type": "xsd:string",
       "@container":"@list"
      },
      "rdfs:comment": "The nationality of the person registered."
    },
    {
      "@id": "spdci:employment_status",
      "@type": "rdfs:Datatype",
      "rdfs:domain": "spdci:Person",
      "rdfs:range": "spdci:EmploymentStatusEnum",
      "rdfs:comment": "Binary representation of if the beneficiary is formally employed or not."
    },
    {
      "@id": "spdci:is_deceased",
      "@type": "rdfs:Datatype",
      "rdfs:domain": "spdci:Person",
      "rdfs:range": "spdci:IsDeceasedEnum",
      "rdfs:comment": "Binary representation of if the beneficiary is deceased or not."
    },
    {
      "@id": "spdci:death_date",
      "@type": "rdfs:Datatype",
      "rdfs:domain": "spdci:Person",
      "rdfs:range": "common:DateTime",
      "rdfs:comment": "The date of birth of the applicant, formatted according to schema:DateTime."
    },
    {
      "@id": "spdci:ethnicity",
      "@type": "rdfs:Datatype",
      "rdfs:domain": "spdci:Person",
      "rdfs:range": {
           "@type": "xsd:string",
           "@container": "@list"
      },
      "rdfs:comment": "Ethnicity of the applicant."
    },
    {
      "@id": "spdci:address",
      "@type": "rdfs:Datatype",
      "rdfs:domain": "spdci:Person",
      "rdfs:range": {
           "@id": "spdci:Address",
           "@type": "rdfs:Class",
           "@container": "@list",
           "minitems": 1
      },
      "rdfs:comment": "Current residential address of the applicant, represented as an address object."
    },
    {
      "@id": "spdci:phone_number",
      "@type": "rdfs:Datatype",
      "rdfs:domain": "spdci:Person",
      "rdfs:range": {
        "@type":  "xsd:string",
        "@container":"@list"
      },
      "rdfs:comment": "Person's preferred phone number. The format E.164 is recommended."
    },
    {
      "@id": "spdci:email",
      "@type": "rdfs:Datatype",
      "rdfs:domain": "spdci:Person",
      "rdfs:range": {
        "@type":  "xsd:string",
        "@container":"@list"
      },
      "rdfs:comment": "Person's preferred email address. The format must comply with RFC 5322 addr-spec."
    },
    {
      "@id": "spdci:household_info",
      "@type": "rdfs:Datatype",
      "rdfs:domain": "common:Household",
      "rdfs:range": {
           "@id": "spdci:Household",
           "@type": "rdfs:Class",
           "@container": "@list",
           "minitems": 1
      },
      "rdfs:comment": "Household information"
    },
    {
      "@id": "spdci:household_status",
      "@type": "rdfs:Datatype",
      "rdfs:domain": "spdci:Person",
      "rdfs:range": "common:HouseholdRoleEnum",
      "rdfs:comment": "Defines the person's role in the household"
    },
    {
      "@id": "spdci:poverty_score",
      "@type": "rdfs:Datatype",
      "rdfs:domain": "spdci:Person",
      "rdfs:range": "xsd:decimal",
      "rdfs:comment": "The poverty score assigned to the household as a result of a proxy means test or other poverty ranking approach."
    },
    {
      "@id": "spdci:parent1_identifier",
      "@type": "rdfs:Datatype",
      "rdfs:domain": "spdci:Person",
      "rdfs:range": "common:Identifier",
      "rdfs:comment": "Identifier for one parent of the applicant. Must be a unique identifier similar to the applicant's identifier."
    },
    {
      "@id": "spdci:parent2_identifier",
      "@type": "rdfs:Datatype",
      "rdfs:domain": "spdci:Person",
      "rdfs:range": "common:Identifier",
      "rdfs:comment": "Identifier for one parent of the applicant. Must be a unique identifier similar to the applicant's identifier."
    },
    {
      "@id": "spdci:registration_date",
      "@type": "rdfs:Datatype",
      "rdfs:domain": "spdci:Person",
      "rdfs:range": "common:DateTime",
      "rdfs:comment": "The date on which the person was first registered in the social registry."
    },
    {
      "@id": "spdci:last_updated",
      "@type": "rdfs:Datatype",
      "rdfs:domain": "spdci:Person",
      "rdfs:range": "common:DateTime",
      "rdfs:comment": "Date on which applicant data was last updated."
    }
  ],
  "required": ["@context","@type","spdci:identifier", "spdci:name", "spdci:birth_date", "spdci:sex", "spdci:is_disabled","spdci:is_deceased","spdci:address","spdci:household_identifier", "spdci:household_status","spdci:poverty_score","spdci:registration_date"]
}
