{
    "@context": {
      "spdci": "https://schema.spdci.org/extensions/social/v1/",
      "rdfs": "http://www.w3.org/2000/01/rdf-schema#",
      "xsd": "http://www.w3.org/2001/XMLSchema#",
      "owl": "http://www.w3.org/2002/07/owl#",
      "common": "https://schema.spdci.org/common/v1/"
    },
    "@id": "spdci:RelatedPerson",
    "@type": "rdfs:Class",
    "rdfs:comment": "This data object contains the information on people and households held in the social registry.",
    "rdfs:label": "RelatedPerson",
    "rdfs:subClassOf": [
      {
        "@type": "rdfs:Class",
        "rdfs:label": "Structured Entity"
      }
    ],
    "rdfs:property": [
      {
        "@id": "spdci:relationship_type",
        "@type": "rdfs:Datatype",
        "rdfs:domain": "spdci:RelatedPerson",
        "rdfs:range": "spdci:RelationshipTypeEnum",
        "rdfs:comment": "The type of relationship a member has with another member of the group."
      },
      {
        "@id": "spdci:related_member_identifier",
        "@type": "rdfs:Datatype",
        "rdfs:domain": "spdci:RelatedPerson",
        "rdfs:range": "xsd:string",
        "rdfs:comment": "A unique identifier assigned to the related household member ."
      }
    ],
    "required": ["@context","@type","spdci:relationship_type","spdci:related_member_identifier"]
  }
  