{
  "@context": {
    "spdci": "https://schema.spdci.org/extensions/social/v1/",
    "rdfs": "http://www.w3.org/2000/01/rdf-schema#",
    "xsd": "http://www.w3.org/2001/XMLSchema#",
    "owl": "http://www.w3.org/2002/07/owl#",
    "common": "https://schema.spdci.org/common/v1/"
  },
  "@id": "spdci:SR_Person",
  "@type": "rdfs:Class",
  "rdfs:comment": "This data object contains the information on people and households held in the social registry.",
  "rdfs:label": "SR Person",
  "rdfs:subClassOf": [
    {
      "@type": "rdfs:Class",
      "rdfs:label": "Structured Entity"
    }
  ],
  "rdfs:property": [
    {
      "@id": "spdci:identifier",
      "@type": "rdfs:Datatype",
      "rdfs:domain": "spdci:SR_Person",
      "rdfs:range": {
           "@id": "common:Identifier",
           "@type": "rdfs:Class",
           "@container": "@list"
      },
      "rdfs:comment": "The person's identification number."
    },
    {
      "@id": "spdci:name",
      "@type": "rdfs:Datatype",
      "rdfs:domain": "spdci:SR_Person",
      "rdfs:range": {
           "@id": "common:Name",
           "@type": "rdfs:Class"
      },
      "rdfs:comment": "Full name in a displayable form, possibly including titles and suffixes, in the order of the applicant's locale norms and/or preferences."
    },
    {
      "@id": "spdci:sex",
      "@type": "rdfs:Datatype",
      "rdfs:domain": "spdci:SR_Person",
      "rdfs:range": "common:SexCategoryEnum",
      "rdfs:comment": "Sex of the applicant, represented as an enumeration ."
    },
    {
      "@id": "spdci:birth_date",
      "@type": "rdfs:Datatype",
      "rdfs:domain": "spdci:SR_Person",
      "rdfs:range": "common:DateTime",
      "rdfs:comment": "The date of birth of the applicant, formatted according to schema:DateTime."
    },
    {
      "@id": "spdci:death_date",
      "@type": "rdfs:Datatype",
      "rdfs:domain": "spdci:SR_Person",
      "rdfs:range": "common:DateTime",
      "rdfs:comment": "The date of birth of the applicant, formatted according to schema:DateTime."
    },
    {
      "@id": "spdci:address",
      "@type": "rdfs:Datatype",
      "rdfs:domain": "spdci:SR_Person",
      "rdfs:range": {
           "@id": "spdci:Address",
           "@type": "rdfs:Class",
           "@container":"@list"
      },
      "rdfs:comment": "Current residential address of the applicant, represented as an address object."
    },
    {
      "@id": "spdci:phone_number",
      "@type": "rdfs:Datatype",
      "rdfs:domain": "spdci:SR_Person",
      "rdfs:range": {
        "@type":  "xsd:string",
        "@container":"@list"
      },
      "rdfs:comment": "Person's preferred phone number. The format E.164 is recommended."
    },
    {
      "@id": "spdci:email",
      "@type": "rdfs:Datatype",
      "rdfs:domain": "spdci:SR_Person",
      "rdfs:range": {
        "@type":  "xsd:string",
        "@container":"@list"
      },
      "rdfs:comment": "Person's preferred email address. The format must comply with RFC 5322 addr-spec."
    },
    {
      "@id": "spdci:registration_date",
      "@type": "rdfs:Datatype",
      "rdfs:domain": "spdci:SR_Person",
      "rdfs:range": "common:DateTime",
      "rdfs:comment": "The date of registration of the applicant, formatted according to schema:DateTime."
    },
    {
      "@id": "spdci:last_updated",
      "@type": "rdfs:Datatype",
      "rdfs:domain": "spdci:SR_Person",
      "rdfs:range": "common:DateTime",
      "rdfs:comment": "The date when person details got updated , formatted according to schema:DateTime."
    }
  ]
}
