{
    "@context": {
      "spdci": "https://schema.spdci.org/extensions/dr/v1/data",
      "code": "https://schema.spdci.org/extensions/dr/v1/code",
      "xsd": "http://www.w3.org/2001/XMLSchema#",
      "spdcicore": "https://schema.spdci.org/core/v1/data",
      "spdcicode": "https://schema.spdci.org/core/v1/code",
      "rdfs": "http://www.w3.org/2000/01/rdf-schema#",
      "owl": "http://www.w3.org/2002/07/owl#"
    },
    "@id": "spdci:DisabilityDetails",
    "@type": "rdfs:Class",
    "rdfs:comment": "This data object contains the information on disabilities a member is suffering from.",
    "rdfs:label": "DisabilityDetails",
    "rdfs:subClassOf": [
      {
        "@type": "rdfs:Class",
        "rdfs:label": "Structured Entity"
      }
    ],
    "rdfs:property": [
          {
            "@id": "spdci:impairment_type",
            "@type": "rdfs:Datatype",
            "rdfs:domain": "spdci:DisabilityDetails",
            "rdfs:range": "code:ImpairmentType",
            "rdfs:comment": "Is the type of impairment the disabled person suffers from."
          },
          {
            "@id": "spdci:impairment_level",
            "@type": "rdfs:Datatype",
            "rdfs:domain": "spdci:DisabilityDetails",
            "rdfs:range": "code:ImpairmentLevel",
            "rdfs:comment": "Is the level of impairment the disabled person suffers from."
          },
          {
            "@id": "spdci:impairment_cause",
            "@type": "rdfs:Datatype",
            "rdfs:domain": "spdci:DisabilityDetails",
            "rdfs:range": "code:ImpairmentCause",
            "rdfs:comment": "Is the cause of impairment the disabled person suffers from."
          },
          {
            "@id": "spdci:age_on_set",
            "@type": "rdfs:Datatype",
            "rdfs:domain": "spdci:DisabilityDetails",
            "rdfs:range": "code:DisabilityOnSet",
            "rdfs:comment": "Is the age when impairment occured."
          }
    ]
    }