{
  "@context": {
    "spdci": "https://schema.spdci.org/extensions/ibr/v1/",
    "rdfs": "http://www.w3.org/2000/01/rdf-schema#",
    "xsd": "http://www.w3.org/2001/XMLSchema#",
    "owl": "http://www.w3.org/2002/07/owl#",
    "openid": "https://schema.spdci.org/extensions/openid/v1/",
    "common": "https://schema.spdci.org/common/v1/"
  },
  "@id": "spdci:Person",
  "@type": "rdfs:Class",
  "rdfs:comment": "Attributes of a person to create fetch records, create verifiable credentials or use in search criteria.",
  "rdfs:label": "Person Record",
  "rdfs:subClassOf": [
    {
      "@type": "rdfs:Class",
      "rdfs:label": "Structured Entity"
    }
  ],
  "rdfs:property": [
    {
      "@id": "spdci:identifier",
      "@type": "rdfs:Datatype",
      "rdfs:domain": "spdci:Person",
      "rdfs:range": {
          "@id": "common:Identifier",
          "@type": "rdfs:Class",
          "@container": "@list"
      },
      "rdfs:comment": "The person's identification number"
    },
    {
      "@id": "spdci:name",
      "@type": "rdfs:Datatype",
      "rdfs:domain": "spdci:Person",
      "rdfs:range": "common:Name",
      "rdfs:comment": "Full name in a displayable form, possibly including titles and suffixes, in the order of the applicant's locale norms and/or preferences."
    },
    {
      "@id": "spdci:household_status",
      "@type": "rdfs:Datatype",
      "rdfs:domain": "spdci:Person",
      "rdfs:range": "spdci:HouseholdStatusEnum"
    },
    {
      "@id": "spdci:benefiting_entity",
      "@type":"rdfs:Datatype",
      "rdfs:domain": "spdci:BenefitingEntity",
      "rdfs:comment": "Defines if the entity benefiting is a person or a household"
    },
    {
      "@id": "spdci:sex",
      "@type": "rdfs:Datatype",
      "rdfs:domain": "spdci:Person",
      "rdfs:range": "common:SexCategoryEnum",
      "rdfs:comment": "Represents the gender of a person."
    },
    {
      "@id": "spdci:birth_date",
      "@type": "rdfs:Datatype",
      "rdfs:domain": "spdci:Person",
      "rdfs:range": "common:DateTime",
      "rdfs:comment": "Birth date of the person"
    },
    {
      "@id": "spdci:sub_region_code",
      "@type": "rdfs:Datatype",
      "rdfs:domain": "spdci:Person",
      "rdfs:range": "common:Address",
      "rdfs:comment": "ISO 3166-2 code and label (eg district or equivalent).  Other more detailed parts of the address are excluded to minimise personal data stored"
    },
    {
      "@id": "spdci:marital_status",
      "@type": "rdfs:Datatype",
      "rdfs:domain": "spdci:Person",
      "rdfs:range": "common:MaritalStatusEnum",
      "rdfs:comment": "Marital status of the person"
    },
    {
      "@id": "spdci:poverty_score",
      "@type": "rdfs:Datatype",
      "rdfs:domain": "spdci:Person",
      "rdfs:range": "xsd:decimal",
      "rdfs:comment": "Household poverty score for the household."
    },
    {
      "@id": "spdci:is_disabled",
      "@type": "rdfs:Datatype",
      "rdfs:domain": "spdci:Person",
      "rdfs:range": "spdci:IsDisabledEnum",
      "rdfs:comment": "Specifies if the person is disabled, not disabled or not known."
    },
    {
      "@id": "spdci:household_identifier",
      "@type": "rdfs:Datatype",
      "rdfs:domain": "spdci:Person",
      "rdfs:range": {
           "@id": "xsd:string",
           "@container": "@list"
      },
      "rdfs:comment": "The identifier for a household that the person is linked to."
    },
    {
      "@id": "spdci:programme",
      "@type": "rdfs:Datatype",
      "rdfs:domain": "spdci:Person",
      "rdfs:range": {
           "@id": "spdci:Programme",
           "@type": "rdfs:Class",
           "@container": "@list"
      },
      "rdfs:comment": "The name for the programme in which the person is/was enrolled and accompanying information"
    },
    {
      "@id": "spdci:benefit",
      "@type": "rdfs:Datatype",
      "rdfs:range": {
           "@id": "spdci:Benefit",
           "@type": "rdfs:Class",
           "@container": "@list"
      },
      "rdfs:comment": "The type of benefit received by the person"
    },
    {
      "@id": "spdci:payroll",
      "@type": "rdfs:Datatype",
      "rdfs:label": "Payroll",
      "rdfs:range": {
           "@id": "spdci:Payroll",
           "@type": "rdfs:Class",
           "@container": "@list"
      },
      "rdfs:comment": "The payroll information for cases where the benefit was provided as a cash transfer"
    }
  ],
  "required": ["@context","@type","spdci:identifier", "spdci:household_status", "spdci:benefiting_entity", "spdci:sub_region_code","spdci:household_identifier", "spdci:programme"]

}


