{
  "@context": {
    "spdci": "http://spdci.org/schemas/src/extensions/ibr/v1/",
    "rdfs": "http://www.w3.org/2000/01/rdf-schema#",
    "xsd": "http://www.w3.org/2001/XMLSchema#",
    "owl": "http://www.w3.org/2002/07/owl#"
  },
  "@id": "spdci:Programme",
  "@type": "rdfs:Class",
  "rdfs:label": "Programme Enrollment",
  "rdfs:subClassOf": [
    {
      "@type": "rdfs:Class",
      "rdfs:label": "Structured Entity"
    }
  ],
  "rdfs:property": [
    {
      "@id": "spdci:programme_name",
      "@type": "rdfs:Datatype",
      "rdfs:domain": "spdci:Programme",
      "rdfs:range": "xsd:string",
      "rdfs:comment": "The programme name sent by the SP system."
    },
    {
      "@id": "spdci:programme_identifier",
      "@type": "rdfs:Datatype",
      "rdfs:domain": "spdci:Programme",
      "rdfs:range": "xsd:string",
      "rdfs:comment": "Programme identifier."
    },
    {
      "@id": "spdci:registration_date",
      "@type": "rdfs:Datatype",
      "rdfs:domain": "spdci:Programme",
      "rdfs:range": "  ",
      "rdfs:comment": "The date when the beneficiary was registered into the programme."
    },
    {
      "@id": "spdci:enrolment_date",
      "@type": "rdfs:Datatype",
      "rdfs:domain": "spdci:Programme",
      "rdfs:range": " ",
      "rdfs:comment": "The date when the beneficiary was enrolled into the programme."
    },
    {
      "@id": "spdci:suspension_date",
      "@type": "rdfs:Datatype",
      "rdfs:domain": "spdci:Programme",
      "rdfs:range": "common:DateTime",
      "rdfs:comment": "The date when the beneficiary was suspended from the programme."
    },
    {
      "@id": "spdci:graduation_date",
      "@type": "rdfs:Datatype",
      "rdfs:domain": "spdci:Programme",
      "rdfs:range": " ",
      "rdfs:comment": "The date when the beneficiary graduated."
    },
    {
      "@id": "spdci:status",
      "@type": "rdfs:Datatype",
      "rdfs:domain": "spdci:Programme",
      "rdfs:range": "benefit:BeneficiaryStatusEnum"
    }
  ]
}
