{
  "@context": {
    "spdci": "https://schema.spdci.org/extensions/ibr/v1/",
    "rdfs": "http://www.w3.org/2000/01/rdf-schema#",
    "xsd": "http://www.w3.org/2001/XMLSchema#",
    "owl": "http://www.w3.org/2002/07/owl#"
  },
  "@id": "spdci:Programme",
  "@type": "rdfs:Class",
  "rdfs:label": "Programme Enrollment",
  "rdfs:subClassOf": [
    {
      "@type": "rdfs:Class",
      "rdfs:label": "Structured Entity"
    }
  ],
  "rdfs:property": [
    {
      "@id": "spdci:programme_name",
      "@type": "rdfs:Datatype",
      "rdfs:domain": "spdci:Programme",
      "rdfs:range": "xsd:string",
      "rdfs:comment": "The name for the programme in which the person is/was enrolled."
    },
    {
      "@id": "spdci:programme_identifier",
      "@type": "rdfs:Datatype",
      "rdfs:domain": "spdci:Programme",
      "rdfs:range": "xsd:string",
      "rdfs:comment": "The identifier for a programme in which the person is/was enrolled."
    },
    {
      "@id": "spdci:programme_description",
      "@type": "rdfs:Datatype",
      "rdfs:domain": "spdci:Programme",
      "rdfs:range": "xsd:string",
      "rdfs:comment": "A description of the programme and it's objectives"
    },
    {
      "@id": "spdci:implementing_institution",
      "@type": "rdfs:Datatype",
      "rdfs:domain": "spdci:Programme",
      "rdfs:range": "xsd:string",
      "rdfs:comment": "A description of the programme and it's objectives"
    },
    {
      "@id": "spdci:institution_type",
      "@type": "rdfs:Datatype",
      "rdfs:domain": "spdci:Programme",
      "rdfs:range": "spdci:InstitutionEnum",
      "rdfs:comment": "The type of institution responsible for implementing the programme"
    },
    {
      "@id": "spdci:legal_status",
      "@type": "rdfs:Datatype",
      "rdfs:domain": "spdci:Programme",
      "rdfs:range": "spdci:LegalStatusEnum",
      "rdfs:comment": "Specifies if the programme is anchored in legislation"
    },
    {
      "@id": "spdci:social_protection_functions",
      "@type": "rdfs:Datatype",
      "rdfs:domain": "spdci:Programme",
      "rdfs:range": {
        "@type": "spdci:SocialProtectionFunctionEnum",
        "@container": "@list"
      },
      "rdfs:comment": "The type of social protection functions provided by the programme.  More than one value may be provided"
    },
    {
      "@id": "spdci:contribution_type",
      "@type": "rdfs:Datatype",
      "rdfs:domain": "spdci:Programme",
      "rdfs:range": "spdci:ContributionTypeEnum",
      "rdfs:comment": "Specifies if a contribution is required by beneficiaries"
    },
    {
      "@id": "spdci:programme_type",
      "@type": "rdfs:Datatype",
      "rdfs:domain": "spdci:Programme",
      "rdfs:range": "spdci:ContributionTypeEnum",
      "rdfs:comment": "Specifies if a contribution is required by beneficiaries"
    },
    {
      "@id": "spdci:benefit",
      "@type": "rdfs:Datatype",
      "rdfs:domain": "spdci:Programme",
      "rdfs:range": {
        "@type": "spdci:Benefit",
        "@container": "@list"
      },
      "rdfs:comment": "The benefits provided by the programme"
    },
    {
      "@id": "spdci:benefit_frequency",
      "@type": "rdfs:Datatype",
      "rdfs:domain": "spdci:Programme",
      "rdfs:range": {
        "@type": "spdci:BenefitFrequency",
        "@container": "@list"
      },
      "rdfs:comment": "The benefits provided by the programme"
    }
  ],
  "required": ["@context","@type", "spdci:programme_name", "spdci:programme_identifier", "spdci:enrolment_date", "spdci:enrolment_status"]
}
