{
  "@context": {
    "spdci": "https://schema.spdci.org/extensions/mosip/v1/",
    "rdfs": "http://www.w3.org/2000/01/rdf-schema#",
    "xsd": "http://www.w3.org/2001/XMLSchema#",
    "owl": "http://www.w3.org/2002/07/owl#"
  },
  "@id": "spdci:RegistrationRecord",
  "@type": "rdfs:Class",
  "rdfs:comment": "Birth Registration record to sync with MOSIP.",
  "rdfs:label": "Registration Record",
  "rdfs:subClassOf": [
    {
      "@type": "rdfs:Class",
      "rdfs:label": "Structured Entity"
    }
  ],
  "rdfs:property": [
    {
      "@id": "spdci:registration_id",
      "@type": "rdfs:Datatype",
      "rdfs:domain": "spdci:RegistrationRecord",
      "rdfs:range": "xsd:string",
      "rdfs:comment": "Unique identifier for the birth registration record."
    },
    {
      "@id": "spdci:packetId",
      "@type": "rdfs:Datatype",
      "rdfs:domain": "spdci:RegistrationRecord",
      "rdfs:range": "xsd:string",
      "rdfs:comment": "Identifier for the packet associated with the birth registration record."
    },
    {
      "@id": "spdci:additional_info_reqId",
      "@type": "rdfs:Datatype",
      "rdfs:domain": "spdci:RegistrationRecord",
      "rdfs:range": "xsd:string",
      "rdfs:comment": "Identifier for additional information request associated with the birth registration record."
    },
    {
      "@id": "spdci:name",
      "@type": "rdfs:Datatype",
      "rdfs:domain": "spdci:RegistrationRecord",
      "rdfs:range": "xsd:string",
      "rdfs:comment": "Name associated with the birth registration record."
    },
    {
      "@id": "spdci:email",
      "@type": "rdfs:Datatype",
      "rdfs:domain": "spdci:RegistrationRecord",
      "rdfs:range": "xsd:string",
      "rdfs:comment": "Email associated with the birth registration record."
    },
    {
      "@id": "spdci:phone",
      "@type": "rdfs:Datatype",
      "rdfs:domain": "spdci:RegistrationRecord",
      "rdfs:range": "xsd:string",
      "rdfs:comment": "Phone number associated with the birth registration record."
    },
    {
      "@id": "spdci:registration_type",
      "@type": "rdfs:Datatype",
      "rdfs:domain": "spdci:RegistrationRecord",
      "rdfs:range": "xsd:string",
      "rdfs:comment": "Type of birth registration."
    },
    {
      "@id": "spdci:packet_hash_value",
      "@type": "rdfs:Datatype",
      "rdfs:domain": "spdci:RegistrationRecord",
      "rdfs:range": "xsd:string",
      "rdfs:comment": "Hash value associated with the packet."
    },
    {
      "@id": "spdci:packet_size",
      "@type": "rdfs:Datatype",
      "rdfs:domain": "spdci:RegistrationRecord",
      "rdfs:range": "xsd:number"
    },
    {
      "@id": "spdci:supervisor_status",
      "@type": "rdfs:Datatype",
      "rdfs:domain": "spdci:RegistrationRecord",
      "rdfs:range": "xsd:string",
      "rdfs:comment": "Status of the supervisor for the birth registration record."
    },
    {
      "@id": "spdci:supervisor_comment",
      "@type": "rdfs:Datatype",
      "rdfs:domain": "spdci:RegistrationRecord",
      "rdfs:range": "xsd:string",
      "rdfs:comment": "Comment provided by the supervisor for the birth registration record."
    },
    {
      "@id": "spdci:optional_values",
      "@type": "rdf:Property",
      "rdfs:domain": "spdci:RegistrationRecord",
      "rdfs:range": {
        "@id": "rdf:List",
        "@type": "rdfs:Class",
        "rdfs:comment": "Optional values associated with the birth registration record.",
        "rdfs:label": "Optional Values",
        "rdfs:member": {
          "@id": "rdf:rest",
          "@type": "rdf:Property",
          "rdf:first": {
            "@id": "rdf:first",
            "@type": "rdfs:Datatype",
            "rdfs:range": "xsd:string"
          },
          "rdf:rest": {
            "@id": "rdf:rest",
            "@type": "rdf:Property"
          }
        }
      }
    },
    {
      "@id": "spdci:lang_code",
      "@type": "rdfs:Datatype",
      "rdfs:domain": "spdci:RegistrationRecord",
      "rdfs:range": "xsd:string",
      "rdfs:comment": "Language code associated with the birth registration record."
    },
    {
      "@id": "spdci:create_date_time",
      "@type": "rdfs:Datatype",
      "rdfs:domain": "spdci:RegistrationRecord",
      "@range": "https://schema.spdci.org/common/schema/DateTime",
      "rdfs:comment": "Date and time when the birth registration record was created."
    },
    {
      "@id": "spdci:update_date_time",
      "@type": "rdfs:Datatype",
      "rdfs:domain": "spdci:RegistrationRecord",
      "@range": "https://schema.spdci.org/common/schema/DateTime",
      "rdfs:comment": "Date and time when the birth registration record was last updated."
    },
    {
      "@id": "spdci:deleted_date_time",
      "@type": "rdfs:Datatype",
      "rdfs:domain": "spdci:RegistrationRecord",
      "@range": "https://schema.spdci.org/common/schema/DateTime",
      "rdfs:comment": "Date and time when the birth registration record was deleted."
    },
    {
      "@id": "spdci:is_active",
      "@type": "rdfs:Datatype",
      "rdfs:domain": "spdci:RegistrationRecord",
      "rdfs:range": "xsd:boolean",
      "rdfs:comment": "Indicator of whether the birth registration record is active."
    },
    {
      "@id": "spdci:is_deleted",
      "@type": "rdfs:Datatype",
      "rdfs:domain": "spdci:RegistrationRecord",
      "rdfs:range": "xsd:boolean",
      "rdfs:comment": "Indicator of whether the birth registration record is deleted."
    }
  ]
}
