{
  "@context": {
    "@vocab": "https://schema.spdci.org/extensions/dci/v1",
    "xsd": "http://www.w3.org/2001/XMLSchema#",
    "common": "https://schema.spdci.org/common/v1/",
    "rdfs": "http://www.w3.org/2000/01/rdf-schema#",
    "owl": "http://www.w3.org/2002/07/owl#"
  },
  "@graph": [
    {
      "rdfs:subClassOf": "rdfs:Resource",
      "@id": "spdci:Person",
      "@type": "rdfs:Class",
      "rdfs:comment": "Represents a person in a Civil Registration and Vital Statistics context.",
      "rdfs:property": [
        {
          "@id": "spdci:identifier",
          "@type": "rdfs:Datatype",
          "rdfs:domain": "spdci:Person",
          "rdfs:range": {
            "@id":"common:Identifier",
          },
          "rdfs:comment": "Applicant's identifier in the CRVS system using URI format."
        },
        {
          "@id": "spdci:name",
          "@type": "rdfs:Datatype",
          "rdfs:domain": "spdci:Person",
          "rdfs:range": "common:Name",
          "rdfs:comment": "Full name in a displayable form, including possible titles and suffixes. Formatted according to the applicant's locale norms and/or preferences."
        },
        {
          "@id": "spdci:phone_number",
          "@type": "rdfs:Datatype",
          "rdfs:domain": "spdci:Person",
          "rdfs:range": "xsd:string",
          "rdfs:comment": "Applicant's preferred phone number. The format E.164 is recommended."
        },
        {
          "@id": "spdci:email",
          "@type": "rdfs:Datatype",
          "rdfs:domain": "spdci:Person",
          "rdfs:range": "xsd:string",
          "rdfs:comment": "Applicant's preferred email address. The format must comply with RFC 5322 addr-spec."
        },
        {
          "@id": "spdci:sex",
          "rdfs:comment": "Sex of the applicant, represented as an enumeration (Male, Female, Others, Unknown).",
          "@type": "rdfs:Datatype",
          "rdfs:domain": "spdci:Person",
          "rdfs:range": {
            "@id": "common:SexCategoryEnum"
           }
        },
        {
          "@id": "spdci:birth_date",
          "rdfs:comment": "The date of birth of the applicant, formatted according to schema:DateTime.",
          "@type": "rdfs:Datatype",
          "rdfs:domain": "spdci:Person",
          "rdfs:range": "common:DateTime"
        },
        {
          "@id": "spdci:birth_place",
          "rdfs:comment": "Physical location where the applicant was born, represented as an address object.",
          "@type": "rdfs:Datatype",
          "rdfs:domain": "spdci:Person",
          "rdfs:range": "common:Place"
        },
        {
          "@id": "spdci:death_date",
          "rdfs:comment": "The date of death of the applicant, if applicable. Formatted according to schema:DateTime.",
          "@type": "rdfs:Datatype",
          "rdfs:domain": "spdci:Person",
          "rdfs:range": "common:DateTime"
        },
        {
          "@id": "spdci:death_place",
          "rdfs:comment": "Physical location where the applicant died, if applicable. Represented as an address object.",
          "@type": "rdfs:Datatype",
          "rdfs:domain": "spdci:Person",
          "rdfs:range": "common:Place"
        },
        {
          "@id": "spdci:address",
          "rdfs:comment": "Current residential address of the applicant, represented as an address object.",
          "@type": "rdfs:Datatype",
          "rdfs:domain": "spdci:Person",
          "rdfs:range": "common:Place"
        },
        {
          "@id": "spdci:marital_status",
          "rdfs:comment": "Current marital status of the applicant, represented as an enumeration (e.g., Married, Divorced, etc.).",
          "@type": "rdfs:Datatype",
          "rdfs:domain": "spdci:Person",
          "rdfs:range": {"@id": "common:MaritalStatusEnum"}
        },
        {
          "@id": "spdci:marriage_date",
          "rdfs:comment": "Date when the applicant got married, if applicable. Formatted according to schema:DateTime.",
          "@type": "rdfs:Datatype",
          "rdfs:domain": "spdci:Person",
          "rdfs:range": "common:DateTime"
        },
        {
          "@id": "spdci:divorce_date",
          "rdfs:comment": "Date when the applicant got divorced, if applicable. Formatted according to schema:DateTime.",
          "@type": "rdfs:Datatype",
          "rdfs:domain": "spdci:Person",
          "rdfs:range": "common:DateTime"
        },
        {
          "@id": "spdci:related_person",
          "@type": "rdfs:ObjectProperty",
          "rdfs:domain": "spdci:Person",
          "rdfs:range": {
            "@id":"spdci:Relationship",
            "@type": "rdfs:Class",
            "@container": "@list"
          },
          "rdfs:comment": "Relationships the applicant has with other persons, represented as an array of relationship objects."
        }
      ]
    }
  ]
}
