{
  "@context": {
    "spdci": "https://schema.spdci.org/extensions/nid/v1/",
    "rdfs": "http://www.w3.org/2000/01/rdf-schema#",
    "xsd": "http://www.w3.org/2001/XMLSchema#",
    "owl": "http://www.w3.org/2002/07/owl#"
  },
  "@id": "spdci:DeceasedRecord",
  "@type": "rdfs:Class",
  "rdfs:comment": "Deceased record obtainable from registries",
  "rdfs:label": "Deceased Record",
  "rdfs:subClassOf": [
    {
      "@type": "rdfs:Class",
      "rdfs:label": "Structured Entity"
    }
  ],
  "rdfs:property": [
    {
      "@id": "spdci:reference_number",
      "@type": "rdfs:Datatype",
      "rdfs:domain": "spdci:DeceasedRecord",
      "rdfs:range": "xsd:string",
      "rdfs:comment": "Unique reference number maintained in the registry for recording death record"
    },
    {
      "@id": "spdci:name",
      "@type": "rdfs:Datatype",
      "rdfs:domain": "spdci:DeceasedRecord",
      "rdfs:range": "xsd:string",
      "rdfs:comment": "End-User's full name in displayable form including all name parts, possibly including titles and suffixes, ordered according to the End-User's locale and preferences"
    },
    {
      "@id": "spdci:gender",
      "@type": "rdfs:Datatype",
      "rdfs:domain": "spdci:DeceasedRecord",
      "rdfs:range": "xsd:string",
      "rdfs:comment": "End-User's gender. Values defined by this specification are female, male, transgender"
    },
    {
      "@id": "spdci:dob",
      "@type": "rdfs:Datatype",
      "rdfs:domain": "spdci:DeceasedRecord",
      "rdfs:range": "xsd:string",
      "rdfs:comment": "Date of Birth in DDMMYYYY format"
    },
    {
      "@id": "spdci:dod",
      "@type": "rdfs:Datatype",
      "rdfs:domain": "spdci:DeceasedRecord",
      "rdfs:range": "xsd:string",
      "rdfs:comment": "Date of Death in DDMMYYYY format"
    },
    {
      "@id": "spdci:reported_date",
      "@type": "rdfs:Datatype",
      "rdfs:domain": "spdci:DeceasedRecord",
      "rdfs:range": "xsd:string",
      "rdfs:comment": "Date in DDMMYYYY format to record on which the death incident reported"
    },
    {
      "@id": "spdci:demo_check_status",
      "@type": "rdfs:Datatype",
      "rdfs:domain": "spdci:DeceasedRecord",
      "rdfs:range": "xsd:boolean",
      "rdfs:comment": "Whether demo check has been undertaken or not"
    },
    {
      "@id": "spdci:demo_check_date",
      "@type": "rdfs:Datatype",
      "rdfs:domain": "spdci:DeceasedRecord",
      "rdfs:range": "xsd:string",
      "rdfs:comment": "Date in DDMMYYYY format to capture the Demo Check Date"
    },
    {
      "@id": "spdci:document",
      "@type": "rdfs:Datatype",
      "rdfs:domain": "spdci:DeceasedRecord",
      "rdfs:range": "spdci:Document",
      "rdfs:comment": "Reference to the document associated with the deceased record"
    }
  ]
}
