{
  "@context": {
    "spdci": "https://schema.spdci.org/extensions/nid/v1/",
    "rdfs": "http://www.w3.org/2000/01/rdf-schema#",
    "xsd": "http://www.w3.org/2001/XMLSchema#",
    "owl": "http://www.w3.org/2002/07/owl#"
  },
  "@id": "spdci:ResidentRecord",
  "@type": "rdfs:Class",
  "rdfs:comment": "Resident Information",
  "rdfs:label": "Resident Information",
  "rdfs:subClassOf": [
    {
      "@type": "rdfs:Class",
      "rdfs:label": "Structured Entity"
    }
  ],
  "rdfs:property": [
    {
      "@id": "spdci:name",
      "@type": "rdfs:Datatype",
      "rdfs:domain": "spdci:ResidentRecord",
      "rdfs:range": "xsd:string",
      "rdfs:comment": "End-User's full name in displayable form including all name parts, possibly including titles and suffixes, ordered according to the End-User's locale and preferences."
    },
    {
      "@id": "spdci:gender",
      "@type": "rdfs:Datatype",
      "rdfs:domain": "spdci:ResidentRecord",
      "rdfs:range": "xsd:string",
      "rdfs:comment": "End-User's gender. Values defined by this specification are female, male, transgender."
    },
    {
      "@id": "spdci:dob",
      "@type": "rdfs:Datatype",
      "rdfs:domain": "spdci:ResidentRecord",
      "rdfs:range": "xsd:string",
      "rdfs:comment": "Date of Birth in DDMMYYYY format"
    },
    {
      "@id": "spdci:dob_type",
      "@type": "rdfs:Datatype",
      "rdfs:domain": "spdci:ResidentRecord",
      "rdfs:range": "xsd:string",
      "rdfs:comment": "Date of Birth Type i.e Declared, Approximate, Verified"
    },
    {
      "@id": "spdci:phone",
      "@type": "rdfs:Datatype",
      "rdfs:domain": "spdci:ResidentRecord",
      "rdfs:range": "xsd:string",
      "rdfs:comment": "Phone number of the resident. If the number contains an extension, it is RECOMMENDED that the extension be represented using the RFC 3966 [RFC3966] extension syntax, for example, +1 (604) 555-1234;ext=5678."
    },
    {
      "@id": "spdci:email",
      "@type": "rdfs:Datatype",
      "rdfs:domain": "spdci:ResidentRecord",
      "rdfs:range": "xsd:string",
      "rdfs:comment": "End-User's preferred e-mail address. Its value MUST conform to the RFC 5322 [RFC5322] addr-spec syntax. The RP MUST NOT rely upon this value being unique, as discussed in Section 5.7."
    },
    {
      "@id": "spdci:address",
      "@type": "rdfs:Datatype",
      "rdfs:domain": "spdci:ResidentRecord",
      "rdfs:range": "spdci:ResidentAddress"
    },
    {
      "@id": "spdci:local_name",
      "@type": "rdfs:Datatype",
      "rdfs:domain": "spdci:ResidentRecord",
      "rdfs:range": "spdci:ResidentLocalName"
    },
    {
      "@id": "spdci:local_address",
      "@type": "rdfs:Datatype",
      "rdfs:domain": "spdci:ResidentRecord",
      "rdfs:range": "spdci:ResidentLocalAddress"
    },
    {
      "@id": "spdci:photo",
      "@type": "rdfs:Datatype",
      "rdfs:domain": "spdci:ResidentRecord",
      "rdfs:range": "spdci:ResidentPhoto"
    },
    {
      "@id": "spdci:nationality",
      "@type": "rdfs:Datatype",
      "rdfs:domain": "spdci:ResidentRecord",
      "rdfs:range": "spdci:ResidentNationality"
    },
    {
      "@id": "spdci:kyc_status",
      "@type": "rdfs:Datatype",
      "rdfs:domain": "spdci:ResidentRecord",
      "rdfs:range": "spdci:EKycDetails"
    },
    {
      "@id": "spdci:document",
      "@type": "rdfs:Datatype",
      "rdfs:domain": "spdci:ResidentRecord",
      "rdfs:range": "spdci:Document"
    }
  ]
}
