{
    "@context": {
      "spdci": "https://schema.spdci.org/extensions/fr/v1/",
      "social": "https://schema.spdci.org/extensions/social/v1/",
      "ibr": "https://schema.spdci.org/extensions/ibr/v1/",
      "rdfs": "http://www.w3.org/2000/01/rdf-schema#",
      "xsd": "http://www.w3.org/2001/XMLSchema#",
      "owl": "http://www.w3.org/2002/07/owl#",
      "common": "https://schema.spdci.org/common/v1/"
    },
    "@id": "spdci:Farming_Activities",
    "@type": "rdfs:Class",
    "rdfs:comment": "This data object contains the information on people  held in the farmer registry",
    "rdfs:label": "Farming_Activities",
    "rdfs:subClassOf": [
      {
        "@type": "rdfs:Class",
        "rdfs:label": "Structured Entity"
      }
    ],
    "rdfs:property": [
        {
            "@id": "spdci:non_perennial_crops",
            "@type": "rdfs:Datatype",
            "rdfs:domain": "spdci:Farming_Activities",
            "rdfs:range": "spdci:CropDetails",
            "rdfs:comment": "Growing of non-perennial crops."
        },
        {
            "@id": "spdci:perennial_crops",
            "@type": "rdfs:Datatype",
            "rdfs:domain": "spdci:Farming_Activities",
            "rdfs:range": "spdci:CropDetails",
            "rdfs:comment": "Growing of perennial crops"
        },
        {
            "@id": "spdci:plant_propagation",
            "@type": "rdfs:Datatype",
            "rdfs:domain": "spdci:Farming_Activities",
            "rdfs:range": "spdci:CropDetails",
            "rdfs:comment": "Plant propagation"
        },
        {
            "@id": "spdci:mixed_farming",
            "@type": "rdfs:Datatype",
            "rdfs:domain": "spdci:Farming_Activities",
            "rdfs:range": "xsd:boolean",
            "rdfs:comment": "Mixed farming, Includes both crops and animal related farming activities"
        },
        {
            "@id": "spdci:agri_support_activities",
            "@type": "rdfs:Datatype",
            "rdfs:domain": "spdci:Farming_Activities",
            "rdfs:range": "spdci:AgriSupportActivityEnum",
            "rdfs:comment": "Support activities to agriculture and post-harvest crop activities"
        },
        {
            "@id": "spdci:aquaculture",
            "@type": "rdfs:Datatype",
            "rdfs:domain": "spdci:Farming_Activities",
            "rdfs:range": "spdci:AquaCultureEnum",
            "rdfs:comment": "Aquaculture"
        },
        {
            "@id": "spdci:aqua_support_activities",
            "@type": "rdfs:Datatype",
            "rdfs:domain": "spdci:Farming_Activities",
            "rdfs:range": "spdci:AquaSupportActivityEnum",
            "rdfs:comment": "Support activities for fishing and aquaculture"
        },
        {
            "@id": "spdci:registration_date",
            "@type": "rdfs:Datatype",
            "rdfs:domain": "spdci:Farming_Activities",
            "rdfs:range": "common:DateTime",
            "rdfs:comment": "The date of registration of the applicant, formatted according to schema:DateTime."
          },
          {
            "@id": "spdci:last_updated",
            "@type": "rdfs:Datatype",
            "rdfs:domain": "spdci:Farming_Activities",
            "rdfs:range": "common:DateTime",
            "rdfs:comment": "The date when person details got updated , formatted according to schema:DateTime."
          }
      
    ]
  }
  