{
    "@context": {
      "spdci": "https://schema.spdci.org/extensions/dr/v1/",
      "social": "https://schema.spdci.org/extensions/social/v1/",
      "rdfs": "http://www.w3.org/2000/01/rdf-schema#",
      "xsd": "http://www.w3.org/2001/XMLSchema#",
      "owl": "http://www.w3.org/2002/07/owl#",
      "common": "https://schema.spdci.org/common/v1/"
    },
    "@id": "spdci:DR_Person",
    "@type": "rdfs:Class",
    "rdfs:comment": "This data object contains the information on people  held in the disabled registry",
    "rdfs:label": "DR_Person",
    "rdfs:subClassOf": [
      {
        "@type": "rdfs:Class",
        "rdfs:label": "Structured Entity"
      }
    ],
    "rdfs:property": [
      {
        "@id": "spdci:personal_details",
        "@type": "rdfs:Datatype",
        "rdfs:domain": "spdci:DR_Person",
        "rdfs:range": "social:Member",
        "rdfs:comment": "The disable person, personal details such as identifier, name ..."
      },
      {
        "@id": "spdci:disability_status",
        "@type": "rdfs:Datatype",
        "rdfs:domain": "spdci:DR_Person",
        "rdfs:range": "spdci:DisabilityStatusEnum",
        "rdfs:comment": "The support needed/received by the disabled person."
      },
      {
        "@id": "spdci:disability_level",
        "@type": "rdfs:Datatype",
        "rdfs:domain": "spdci:DR_Person",
        "rdfs:range": "spdci:DisabilityLevelEnum",
        "rdfs:comment": "The support needed/received by the disabled person."
      },
      {
        "@id": "spdci:disability_details",
        "@type": "rdfs:Datatype",
        "rdfs:domain": "spdci:DR_Person",
        "rdfs:range": {
          "@id": "spdci:DisabilityDetails",
          "@type": "rdfs:Class",
          "@container": "@list"
        },
        "rdfs:comment": "Is the disability details of the person"
      },
      {
        "@id": "spdci:disability_support",
        "@type": "rdfs:Datatype",
        "rdfs:domain": "spdci:DR_Person",
        "rdfs:range": {
          "@id": "spdci:DisabilitySupport",
          "@type": "rdfs:Class",
          "@container": "@list"
        },
        "rdfs:comment": "Is the disability support of the person"
      },
      {
        "@id": "spdci:transport_requirement",
        "@type": "rdfs:Datatype",
        "rdfs:domain": "spdci:DR_Person",
        "rdfs:range": "spdci:TransportRequirement",
        "rdfs:comment": "The support needed for transportation by the disabled person."
      },
      {
        "@id": "spdci:housing_type",
        "@type": "rdfs:Datatype",
        "rdfs:domain": "spdci:DR_Person",
        "rdfs:range": "spdci:HousingType",
        "rdfs:comment": "The house where the disabled person currently in."
      },
      {
        "@id": "spdci:registration_date",
        "@type": "rdfs:Datatype",
        "rdfs:domain": "spdci:DR_Person",
        "rdfs:range": "common:DateTime",
        "rdfs:comment": "The date of registration of the applicant, formatted according to schema:DateTime."
      },
      {
        "@id": "spdci:last_updated",
        "@type": "rdfs:Datatype",
        "rdfs:domain": "spdci:DR_Person",
        "rdfs:range": "common:DateTime",
        "rdfs:comment": "The date when person details got updated , formatted according to schema:DateTime."
      }
      
    ]
  }
  