{
    "@context": {
      "spdci": "https://schema.spdci.org/extensions/dr/v1/",
      "rdfs": "http://www.w3.org/2000/01/rdf-schema#",
      "xsd": "http://www.w3.org/2001/XMLSchema#",
      "owl": "http://www.w3.org/2002/07/owl#",
      "common": "https://schema.spdci.org/common/v1/"
    },
    "@id": "spdci:MedicalCare",
    "@type": "rdfs:Class",
    "rdfs:comment": "This data object contains the information on medical care a member needs",
    "rdfs:label": "MedicalCare",
    "rdfs:subClassOf": [
      {
        "@type": "rdfs:Class",
        "rdfs:label": "Structured Entity"
      }
    ],
    "rdfs:property": [
          {
            "@id": "spdci:type",
            "@type": "rdfs:Datatype",
            "rdfs:domain": "spdci:MedicalCare",
            "rdfs:range": "spdci:MedicalCareEnum",
            "rdfs:comment": "Is the type of medical care the disabled person will need."
          },
          {
            "@id": "spdci:status",
            "@type": "rdfs:Datatype",
            "rdfs:domain": "spdci:MedicalCare",
            "rdfs:range": "spdci:SupportStatusEnum",
            "rdfs:comment": "Is the status if recieved or still needed."
          },
          {

            "@id": "spdci:registration_date",
            "@type": "rdfs:Datatype",
            "rdfs:domain": "spdci:MedicalCare",
            "rdfs:range": "common:DateTime",
            "rdfs:comment": "The date of registration of the applicant, formatted according to schema:DateTime."
          },
          {
            "@id": "spdci:last_updated",
            "@type": "rdfs:Datatype",
            "rdfs:domain": "spdci:MedicalCare",
            "rdfs:range": "common:DateTime",
            "rdfs:comment": "The date when person details got updated , formatted according to schema:DateTime."
          }
          
    ]
    }