{
    "@context": {
      "spdci": "https://schema.spdci.org/extensions/dr/v1/",
      "social": "https://schema.spdci.org/extensions/social/v1/",
      "rdfs": "http://www.w3.org/2000/01/rdf-schema#",
      "xsd": "http://www.w3.org/2001/XMLSchema#",
      "owl": "http://www.w3.org/2002/07/owl#",
      "common": "https://schema.spdci.org/common/v1/"
    },
    "@id": "spdci:Treatment",
    "@type": "rdfs:Class",
    "rdfs:comment": "This data object contains the information on hospital a disabled member is being treated in",
    "rdfs:label": "Treatment",
    "rdfs:subClassOf": [
      {
        "@type": "rdfs:Class",
        "rdfs:label": "Structured Entity"
      }
    ],
    "rdfs:property": [
        {
            "@id": "spdci:hospital",
            "@type": "rdfs:Datatype",
            "rdfs:domain": "spdci:Treatment",
            "rdfs:range": "xsd:string",
            "rdfs:comment": "hospital name member getting treatment in."
          },
          {
            "@id": "spdci:address",
            "@type": "rdfs:Datatype",
            "rdfs:domain": "spdci:Treatment",
            "rdfs:range": {
                 "@id": "spdci:Address",
                 "@type": "rdfs:Class"
            },
            "rdfs:comment": "Hospital address."
          },
          {
            "@id": "spdci:treating_doctor",
            "@type": "rdfs:Datatype",
            "rdfs:domain": "spdci:Treatment",
            "rdfs:range": "social:Person",
            "rdfs:comment": "The doctor treating the Disabled person"
          },
          {
            "@id": "spdci:treatment_type",
            "@type": "rdfs:Datatype",
            "rdfs:domain": "spdci:Treatment",
            "rdfs:range": "xsd:string",
            "rdfs:comment": "general description of the type of treatment being administered (e.g., surgery, rehabilitation)."
          },
          {
            "@id": "spdci:treatment_status",
            "@type": "rdfs:Datatype",
            "rdfs:domain": "spdci:Treatment",
            "rdfs:range": "xsd:string",
            "rdfs:comment": "An indicator of the current status of the treatment (e.g., ongoing, completed, discharged)."
          },
          {
            "@id": "spdci:treatment_start_date",
            "@type": "rdfs:Datatype",
            "rdfs:range": "xsd:DateTime",
            "rdfs:comment": "Date on which applicant started treatment."
          },
          {
            "@id": "spdci:treatment_end_date",
            "@type": "rdfs:Datatype",
            "rdfs:range": "xsd:DateTime",
            "rdfs:comment": "Date on which applicant ended treatment."
          }
    ],
    "required": ["@context","@type","spdci:treating_doctor","spdci:treatment_status","spdci:treatment_start_date"]
  }